Enhanced discrimination nets implementation, which can now work with goals containing existentials and use transparency information on constants (optionally). Only used by the typeclasses eauto engine for now, but could be used for other hint bases easily (just switch a boolean). Had to add a new "creation" hint to be able to set said boolean upon creation of the typeclass_instances hint db. Improve the proof-search algorithm for Morphism, up to 10 seconds gained in e.g. Field_theory, Ring_polynom. Added a morphism declaration for [compose]. One needs to declare more constants as being unfoldable using the [Typeclasses unfold] command so that discrimination is done correctly, but that amounts to only 6 declarations in the standard library.
git-svn-id: svn+ssh://scm.gforge.inria.fr/svn/coq/trunk@11184 85f007b7-540e-0410-9357-904b9bb8a0f7

contrib/funind/functional_principles_proofs.ml
@@ -1399,7 +1399,7 @@ let new_prove_with_tcc is_mes acc_inv hrec tcc_hyps eqs : tactic =
 				      false
 				      (true,5)
 				      [Lazy.force refl_equal]
-				      [empty_transparent_state, Auto.Hint_db.empty]
+				      [Auto.Hint_db.empty false]
 				  )
 			   )
 			)
