tactics/auto.mli
@@ -47,24 +47,30 @@ type search_entry = stored_data list * stored_data list * stored_data Btermdn.t
 module Hint_db :
   sig
     type t
-    val empty : t
+    val empty : bool -> t
     val find : global_reference -> t -> search_entry
     val map_all : global_reference -> t -> pri_auto_tactic list
     val map_auto : global_reference * constr -> t -> pri_auto_tactic list
     val add_one : global_reference * pri_auto_tactic -> t -> t
     val add_list : (global_reference * pri_auto_tactic) list -> t -> t
     val iter : (global_reference -> stored_data list -> unit) -> t -> unit
+
+    val transparent_state : t -> transparent_state
+    val set_transparent_state : t -> transparent_state -> t
+    val set_rigid : t -> constant -> t
   end
 
 type hint_db_name = string
 
-type hint_db = transparent_state * Hint_db.t
+type hint_db = Hint_db.t
 
 val searchtable_map : hint_db_name -> hint_db
 
-val current_db_names : unit -> hint_db_name list
+val searchtable_add : (hint_db_name * hint_db) -> unit
 
-val add_hint_list : (global_reference * pri_auto_tactic) list -> hint_db -> hint_db
+val create_hint_db : bool -> hint_db_name -> bool -> unit
+
+val current_db_names : unit -> hint_db_name list
 
 val add_hints : locality_flag -> hint_db_name list -> hints -> unit
 
@@ -207,3 +213,5 @@ val superauto : int -> (identifier * constr) list -> autoArguments list -> tacti
 *)
 
 val h_superauto : int option -> reference list -> bool -> bool -> tactic
+
+val auto_init : (unit -> unit) ref
