tactics/btermdn.mli
@@ -11,6 +11,7 @@
 (*i*)
 open Term
 open Pattern
+open Names
 (*i*)
 
 (* Discrimination nets with bounded depth. *)
@@ -19,10 +20,10 @@ type 'a t
 
 val create : unit -> 'a t
 
-val add : 'a t -> (constr_pattern * 'a) -> 'a t
-val rmv : 'a t -> (constr_pattern * 'a) -> 'a t
-
-val lookup : 'a t -> constr -> (constr_pattern * 'a) list
+val add : transparent_state option -> 'a t -> (constr_pattern * 'a) -> 'a t
+val rmv : transparent_state option -> 'a t -> (constr_pattern * 'a) -> 'a t
+  
+val lookup : transparent_state option -> 'a t -> constr -> (constr_pattern * 'a) list
 val app : ((constr_pattern * 'a) -> unit) -> 'a t -> unit
 
 val dnet_depth : int ref
