theories/Classes/Morphisms.v
@@ -39,10 +39,6 @@ Class Morphism A (R : relation A) (m : A) : Prop :=
 
 Implicit Arguments Morphism [A].
 
-(** We allow to unfold the [relation] definition while doing morphism search. *)
-
-Typeclasses unfold relation.
-
 (** Respectful morphisms. *)
 
 (** The fully dependent version, not used yet. *)
@@ -79,6 +75,15 @@ Arguments Scope respectful [type_scope type_scope signature_scope signature_scop
 
 Open Local Scope signature_scope.
 
+(** Pointwise lifting is just respect with leibnize equality on the left. *)
+
+Definition pointwise_relation {A B : Type} (R : relation B) : relation (A -> B) := 
+  fun f g => forall x : A, R (f x) (g x).
+
+Lemma pointwise_pointwise A B (R : relation B) : 
+  relation_equivalence (pointwise_relation R) (@eq A ==> R).
+Proof. intros. split. simpl_relation. firstorder. Qed.
+
 (** We can build a PER on the Coq function space if we have PERs on the domain and
    codomain. *)
 
@@ -99,17 +104,18 @@ Proof. firstorder. Qed.
 
 (** The subrelation property goes through products as usual. *)
 
-Instance morphisms_subrelation [ sub : subrelation A R₁ R₂ ] :
-  ! subrelation (B -> A) (R ==> R₁) (R ==> R₂).
-Proof. firstorder. Qed.
+Instance morphisms_subrelation_respectful [ subl : subrelation A R₂ R₁, subr : subrelation B S₁ S₂ ] :
+  subrelation (R₁ ==> S₁) (R₂ ==> S₂).
+Proof. simpl_relation. apply subr. apply H. apply subl. apply H0. Qed.
 
-Instance morphisms_subrelation_left [ sub : subrelation A R₂ R₁ ] :
-  ! subrelation (A -> B) (R₁ ==> R) (R₂ ==> R) | 3.
-Proof. firstorder. Qed.
+(** And of course it is reflexive. *)
+
+Instance morphisms_subrelation_refl : ! subrelation A R R | 10.
+Proof. simpl_relation. Qed.
 
 (** [Morphism] is itself a covariant morphism for [subrelation]. *)
 
-Lemma subrelation_morphism [ sub : subrelation A R₁ R₂, mor : Morphism A R₁ m ] : Morphism R₂ m.
+Lemma subrelation_morphism [ mor : Morphism A R₁ m, sub : subrelation A R₁ R₂ ] : Morphism R₂ m.
 Proof.
   intros. apply sub. apply mor.
 Qed.
@@ -121,8 +127,9 @@ Proof. reduce. subst. firstorder. Qed.
 (** We use an external tactic to manage the application of subrelation, which is otherwise
    always applicable. We allow its use only once per branch. *)
 
-Inductive subrelation_done : Prop :=
-  did_subrelation : subrelation_done.
+Inductive subrelation_done : Prop := did_subrelation : subrelation_done.
+
+Inductive normalization_done : Prop := did_normalization.
 
 Ltac subrelation_tac := 
   match goal with
@@ -131,7 +138,7 @@ Ltac subrelation_tac :=
       set(H:=did_subrelation) ; eapply @subrelation_morphism
   end.
 
-Hint Extern 4 (@Morphism _ _ _) => subrelation_tac : typeclass_instances.
+Hint Extern 5 (@Morphism _ _ _) => subrelation_tac : typeclass_instances.
 
 (** Essential subrelation instances for [iff], [impl] and [pointwise_relation]. *)
 
@@ -181,20 +188,10 @@ Program Instance trans_contra_co_morphism
     transitivity x0...
   Qed.
 
-(* (** Dually... *) *)
-
-(* Program Instance [ Transitive A R ] => *)
-(*   trans_co_contra_inv_impl_morphism : Morphism (R ++> R --> inverse impl) R. *)
-  
-(*   Next Obligation. *)
-(*   Proof with auto. *)
-(*     apply* trans_contra_co_morphism ; eauto. eauto. *)
-(*   Qed. *)
-
 (** Morphism declarations for partial applications. *)
 
 Program Instance trans_contra_inv_impl_morphism
-  [ Transitive A R ] : Morphism (R --> inverse impl) (R x).
+  [ Transitive A R ] : Morphism (R --> inverse impl) (R x) | 3.
 
   Next Obligation.
   Proof with auto.
@@ -202,7 +199,7 @@ Program Instance trans_contra_inv_impl_morphism
   Qed.
 
 Program Instance trans_co_impl_morphism
-  [ Transitive A R ] : Morphism (R ==> impl) (R x).
+  [ Transitive A R ] : Morphism (R ==> impl) (R x) | 3.
 
   Next Obligation.
   Proof with auto.
@@ -210,23 +207,23 @@ Program Instance trans_co_impl_morphism
   Qed.
 
 Program Instance trans_sym_co_inv_impl_morphism
-  [ Transitive A R, Symmetric A R ] : Morphism (R ==> inverse impl) (R x).
+  [ PER A R ] : Morphism (R ==> inverse impl) (R x) | 2.
 
   Next Obligation.
   Proof with auto.
-    transitivity y...
+    transitivity y... symmetry...
   Qed.
 
 Program Instance trans_sym_contra_impl_morphism
-  [ Transitive A R, Symmetric _ R ] : Morphism (R --> impl) (R x).
+  [ PER A R ] : Morphism (R --> impl) (R x) | 2.
 
   Next Obligation.
   Proof with auto.
-    transitivity x0...
+    transitivity x0... symmetry...
   Qed.
 
 Program Instance equivalence_partial_app_morphism
-  [ Equivalence A R ] : Morphism (R ==> iff) (R x).
+  [ Equivalence A R ] : Morphism (R ==> iff) (R x) | 1.
 
   Next Obligation.
   Proof with auto.
@@ -240,36 +237,16 @@ Program Instance equivalence_partial_app_morphism
    to get an [R y z] goal. *)
 
 Program Instance trans_co_eq_inv_impl_morphism
-  [ Transitive A R ] : Morphism (R ==> (@eq A) ==> inverse impl) R.
+  [ Transitive A R ] : Morphism (R ==> (@eq A) ==> inverse impl) R | 2.
 
   Next Obligation.
   Proof with auto.
     transitivity y...
   Qed.
 
-(* Program Instance [ Transitive A R ] =>  *)
-(*   trans_contra_eq_impl_morphism : Morphism (R --> (@eq A) ==> impl) R. *)
-
-(*   Next Obligation. *)
-(*   Proof with auto. *)
-(*     transitivity x... *)
-(*   Qed. *)
-
 (** Every Symmetric and Transitive relation gives rise to an equivariant morphism. *)
 
-Program Instance trans_sym_morphism
-  [ Transitive A R, Symmetric _ R ] : Morphism (R ==> R ==> iff) R.
-
-  Next Obligation.
-  Proof with auto.
-    split ; intros.
-    transitivity x0... transitivity x...
-  
-    transitivity y... transitivity y0... 
-  Qed.
-
-Program Instance equiv_morphism [ Equivalence A R ] :
-  Morphism (R ==> R ==> iff) R.
+Program Instance PER_morphism [ PER A R ] : Morphism (R ==> R ==> iff) R | 1.
 
   Next Obligation.
   Proof with auto.
@@ -293,6 +270,15 @@ Program Instance iff_impl_id :
 Program Instance inverse_iff_impl_id :
   Morphism (iff --> impl) id.
   
+Program Instance compose_morphism A B C R₀ R₁ R₂ :
+  Morphism ((R₁ ==> R₂) ==> (R₀ ==> R₁) ==> (R₀ ==> R₂)) (@compose A B C).
+
+  Next Obligation.
+  Proof.
+    simpl_relation.
+    unfold compose. apply H. apply H0. apply H1.
+  Qed.
+
 (** Coq functions are morphisms for leibniz equality, 
    applied only if really needed. *)
 
@@ -342,10 +328,6 @@ Instance morphism_morphism_proxy
   [ Morphism A R x ] : MorphismProxy A R x | 2.
 Proof. firstorder. Qed.
 
-(* Instance (A : Type) [ Reflexive B R ] => *)
-(*   eq_reflexive_morphism : Morphism (@Logic.eq A ==> R) m | 3. *)
-(* Proof. simpl_relation. Qed. *)
-
 (** [R] is Reflexive, hence we can build the needed proof. *)
 
 Lemma Reflexive_partial_app_morphism [ Morphism (A -> B) (R ==> R') m, MorphismProxy A R x ] :
@@ -373,11 +355,10 @@ Ltac partial_application_tactic :=
     end
   in
   match goal with
+    | [ _ : subrelation_done |- _ ] => fail 1
+    | [ _ : normalization_done |- _ ] => fail 1      
     | [ |- @Morphism _ _ ?m ] => on_morphism m
   end.
-
-(* Program Instance [ Morphism (A -> B) (R ==> R') m, Reflexive A R ] (x : A) => *)
-(*   reflexive_partial_app_morphism : Morphism R' (m x). *)
 
 Hint Extern 4 (@Morphism _ _ _) => partial_application_tactic : typeclass_instances.
 
@@ -406,8 +387,8 @@ Proof. firstorder. Qed.
 
 Instance inverse_respectful_rec_norm [ Normalizes B R' (inverse R'') ] :
   Normalizes (A -> B) (inverse R ==> R') (inverse (R ==> R'')).
-Proof. red ; intros.  
-  pose normalizes as r.
+Proof. red ; intros. 
+  assert(r:=normalizes).
   setoid_rewrite r.
   setoid_rewrite inverse_respectful.
   reflexivity.
@@ -415,8 +396,14 @@ Qed.
 
 (** Once we have normalized, we will apply this instance to simplify the problem. *)
 
-Program Instance morphism_inverse_morphism
-  [ Morphism A R m ] : Morphism (inverse R) m | 2.
+Definition morphism_inverse_morphism [ mor : Morphism A R m ] : Morphism (inverse R) m := mor.
+
+Ltac morphism_inverse :=
+  match goal with
+    [ |- @Morphism _ (flip _) _ ] => eapply @morphism_inverse_morphism
+  end.
+
+Hint Extern 2 (@Morphism _ _ _) => morphism_inverse : typeclass_instances.
 
 (** Bootstrap !!! *)
 
@@ -441,10 +428,9 @@ Proof.
   assumption.
 Qed.
 
-Inductive normalization_done : Prop := did_normalization.
-
 Ltac morphism_normalization := 
   match goal with
+    | [ _ : subrelation_done |- _ ] => fail 1
     | [ _ : normalization_done |- _ ] => fail 1
     | [ |- @Morphism _ _ _ ] => let H := fresh "H" in
       set(H:=did_normalization) ; eapply @morphism_releq_morphism
@@ -465,4 +451,4 @@ Ltac morphism_reflexive :=
     | [ |- @Morphism _ _ _ ] => eapply @reflexive_morphism
   end.
 
-Hint Extern 4 (@Morphism _ _ _) => morphism_reflexive : typeclass_instances.
+Hint Extern 7 (@Morphism _ _ _) => morphism_reflexive : typeclass_instances.
