theories/Numbers/Integer/BigZ/BigZ.v
@@ -102,6 +102,8 @@ exact sub_opp.
 exact add_opp.
 Qed.
 
+Typeclasses unfold NZadd NZmul NZsub NZeq.
+
 Add Ring BigZr : BigZring.
 
 (** Todo: tactic translating from [BigZ] to [Z] + omega *)
